Contains Duplicate - Draft

Majority Element/majority_element.dfy
@@ -1,6 +1,6 @@
 method majority_element(nums: array<int>) returns (majority: int)
     requires nums.Length > 0
-    requires exists element :: (count_occurrence(nums, 0, nums.Length - 1, element) > nums.Length / 2)
+    requires exists i :: (0 <= i < nums.Length ==> count_occurrence(nums, 0, nums.Length - 1, nums[i]) > nums.Length / 2)
     // TODO:
     ensures count_occurrence(nums, 0, nums.Length - 1, majority) > nums.Length / 2
 {
@@ -34,13 +34,13 @@ method majority_element(nums: array<int>) returns (majority: int)
     }
 }
 
-function count_occurrence(arr: array<int>, begin: int, end: int, element: int): int
-    requires 0 <= begin <= arr.Length
-    requires 0 <= end <= arr.Length - 1
+function count_occurrence(nums: array<int>, begin: int, end: int, element: int): int
+    requires 0 <= begin <= nums.Length
+    requires 0 <= end <= nums.Length - 1
     decreases end - begin
-    reads arr
+    reads nums
 {
     if begin > end then 0
-    else if arr[begin] == element then 1 + count_occurrence(arr, begin + 1, end, element)
-    else count_occurrence(arr, begin + 1, end, element)
+    else if nums[begin] == element then 1 + count_occurrence(nums, begin + 1, end, element)
+    else count_occurrence(nums, begin + 1, end, element)
 }
