Contains Duplicate/contains_duplicate.dfy
@@ -1,0 +1,44 @@
+method contains_duplicate(nums: array<int>) returns (s: set<int>)
+    requires 1 <= nums.Length <= 100000
+    requires forall i :: 0 <= i < nums.Length ==> -1000000000 <= nums[i] <= 1000000000
+    ensures |s| == nums.Length ==> is_distinct(nums, 0, nums.Length)
+    ensures |s| != nums.Length  ==> exists i :: (0 <= i < nums.Length ==> count_occurrence(nums, 0, nums.Length - 1, nums[i]) >= 2)
+{
+    s := {nums[0]};
+    var length := nums.Length;
+    
+    var i := 1;
+    while (i < length)
+        invariant 1 <= i <= length
+        invariant |s| <= i
+        invariant |s| == i ==> is_distinct(nums, 0, i)
+        invariant |s| < i ==> exists j :: (0 <= j < i ==> count_occurrence(nums, 0, j, nums[j]) >= 2)
+    {
+        s := s + {nums[i]};
+
+        i := i + 1;
+    }    
+}
+
+
+// Helper function
+function count_occurrence(nums: array<int>, begin: int, end: int, element: int): int
+    requires 0 <= begin <= nums.Length
+    requires 0 <= end <= nums.Length - 1
+    decreases end - begin
+    reads nums
+{
+    if begin > end then 0
+    else if nums[begin] == element then 1 + count_occurrence(nums, begin + 1, end, element)
+    else count_occurrence(nums, begin + 1, end, element)
+}
+
+
+// Helper predicate
+predicate is_distinct(nums: array<int>, begin: int, end: int)
+    requires 0 <= begin <= nums.Length
+    requires 0 <= end <= nums.Length
+    reads nums
+{
+    forall i, j :: begin <= i < j < end ==> nums[i] != nums[j]
+}
